SCP-918 - Start drafting proof of completeness of static analysis (#95)
* Add Let shadowing warning
* Draft and start proving completeness of static analysis

isabelle/StaticAnalysis.thy
@@ -1,5 +1,5 @@
 theory StaticAnalysis
-  imports Semantics MList "HOL-Library.Monad_Syntax" HOL.Wellfounded
+  imports Semantics MList "HOL-Library.Monad_Syntax" HOL.Wellfounded SingleInputTransactions
 begin
 
 (* Symbolic mock definition *)
@@ -9,8 +9,8 @@ record SymbolicMonadData = numSymbolicVars :: nat
 
 datatype 'a Symbolic = Symbolic "SymbolicMonadData \<Rightarrow> ('a \<times> SymbolicMonadData) option"
 
-fun execute :: "'a Symbolic \<Rightarrow> SymbolicMonadData \<Rightarrow> ('a \<times> SymbolicMonadData) option" where
-"execute (Symbolic f) = f"
+primrec execute :: "'a Symbolic \<Rightarrow> SymbolicMonadData \<Rightarrow> ('a \<times> SymbolicMonadData) option" where
+  "execute (Symbolic f) = f"
 
 fun bind :: "'a Symbolic \<Rightarrow> ('a \<Rightarrow> 'b Symbolic) \<Rightarrow> 'b Symbolic" where
   "bind m nf =
@@ -28,7 +28,8 @@ fun maybeNth :: "'a list => nat => 'a option" (infixl "!?" 100) where
 definition newVar :: "int Symbolic" where
   "newVar = Symbolic (\<lambda> st . let nsv = numSymbolicVars st in
                    case (symbolicVarValues st) !? nsv of
-                     Some x \<Rightarrow> Some (x, st \<lparr> numSymbolicVars := Suc nsv \<rparr> ) )"
+                     Some x \<Rightarrow> Some (x, st \<lparr> numSymbolicVars := Suc nsv \<rparr> )
+                   | None \<Rightarrow> None )"
 
 fun constrain :: "bool \<Rightarrow> unit Symbolic" where
   "constrain val = Symbolic (\<lambda> st . if val then Some ((), st) else None)"
@@ -73,7 +74,7 @@ function (sequential) generateSymbolicInterval :: "int option \<Rightarrow> (int
 "generateSymbolicInterval None =
   do { hs \<leftarrow> newVar;
        ls \<leftarrow> newVar;
-       constrain (ls < hs);
+       constrain (ls \<le> hs);
        return (ls, hs) }" |
 "generateSymbolicInterval (Some ms) =
   do { (ls, hs) \<leftarrow> generateSymbolicInterval None;
@@ -194,7 +195,7 @@ fun addTransaction :: "int \<Rightarrow> int \<Rightarrow> SymInput option \<Rig
   let prevSymInp = symInput symState in
   let oldPos = whenPos symState in
   do { let tim = slotTim;
-       constrain (newLowSlot < newHighSlot);
+       constrain (newLowSlot \<le> newHighSlot);
        let conditions = (((oldHighSlot < tim) \<or>
                           ((oldLowSlot = newLowSlot) \<and> (oldHighSlot = newHighSlot))) \<and>
                          (newLowSlot \<ge> tim));
@@ -319,7 +320,7 @@ function (sequential) isValidAndFailsAux :: "bool \<Rightarrow> Contract \<Right
   do { let concVal = symEvalVal val (SymState sState);
        let newBVMap = MList.insert valId concVal (symBoundValues sState);
        let newSState = SymState (sState \<lparr> symBoundValues := newBVMap \<rparr>);
-       isValidAndFailsAux hasErr cont newSState }" |
+       isValidAndFailsAux ((member valId (symBoundValues sState)) \<or> hasErr) cont newSState }" |
 "isValidAndFailsAux hasErr (Assert obs cont) sState =
   (let obsVal = symEvalObs obs sState in
    isValidAndFailsAux (hasErr \<or> (\<not> obsVal)) cont sState)" |
@@ -390,12 +391,123 @@ fun hasWarnings :: "TransactionOutput \<Rightarrow> bool" where
 "hasWarnings (TransactionError _) = False" |
 "hasWarnings (TransactionOutput txOutRec) = (Nil \<noteq> txOutWarnings txOutRec)"
 
-theorem staticAnalysisWorks : "(\<exists> t env. execute (wrapper c t (Some st)) x \<noteq> None) =
+fun isCounterExample :: "(bool \<times> SymbolicMonadData) option \<Rightarrow> bool" where
+"isCounterExample None = False" |
+"isCounterExample (Some (b, _)) = b"
+
+theorem noCounterExamplePropagatesComputeEmptyTransaction :
+   "computeTransaction \<lparr> interval = (lo, hi), inputs = [] \<rparr> st c = TransactionOutput \<lparr>txOutWarnings = [], txOutPayments = newPays, txOutState = newSta, txOutContract = newCont\<rparr> \<Longrightarrow>
+     (\<And>t x. \<not> isCounterExample (execute (wrapper c t (Some st)) x)) \<Longrightarrow> isCounterExample (execute (wrapper newCont t2 (Some newSta)) x2) \<Longrightarrow> False"
+  oops
+
+theorem noCounterExamplePropagatesComputeSingleInputTransaction :
+   "computeTransaction \<lparr> interval = (lo, hi), inputs = [inp] \<rparr> st c = TransactionOutput \<lparr>txOutWarnings = [], txOutPayments = newPays, txOutState = newSta, txOutContract = newCont\<rparr> \<Longrightarrow>
+     (\<And>t x. \<not> isCounterExample (execute (wrapper c t (Some st)) x)) \<Longrightarrow> isCounterExample (execute (wrapper newCont t2 (Some newSta)) x2) \<Longrightarrow> False"
+  oops
+
+theorem computeEmptyTransactionWarningIsCounterExample :
+   "(\<And>t2 x. \<not> isCounterExample (execute (wrapper c t2 (Some st)) x)) \<Longrightarrow>
+    computeTransaction \<lparr> interval = (lo, hi), inputs = [] \<rparr> st c = TransactionOutput \<lparr>txOutWarnings = newWarn, txOutPayments = newPays, txOutState = newSta, txOutContract = newCont\<rparr> \<Longrightarrow>
+    newWarn = []"
+  oops
+
+theorem computeSingleInputTransactionWarningIsCounterExample :
+   "(\<And>t2 x. \<not> isCounterExample (execute (wrapper c t2 (Some st)) x)) \<Longrightarrow>
+    computeTransaction \<lparr> interval = (lo, hi), inputs = [inp] \<rparr> st c = TransactionOutput \<lparr>txOutWarnings = newWarn, txOutPayments = newPays, txOutState = newSta, txOutContract = newCont\<rparr> \<Longrightarrow>
+    newWarn = []"
+  oops
+
+lemma staticAnalysisComplete_emptyTransaction : "(\<And>c st p.
+        (\<And>t2 x. \<not> isCounterExample (execute (wrapper c t2 (Some st)) x)) \<Longrightarrow>
+        hasWarnings (playTraceAux \<lparr>txOutWarnings = [], txOutPayments = p, txOutState = st, txOutContract = c\<rparr> t) \<Longrightarrow> False) \<Longrightarrow>
+    (\<And>t2 x. \<not> isCounterExample (execute (wrapper c t2 (Some st)) x)) \<Longrightarrow>
+    hasWarnings (playTraceAux \<lparr>txOutWarnings = newWarns, txOutPayments = p @ newPays, txOutState = newSta, txOutContract = newCont\<rparr> t) \<Longrightarrow>
+    computeTransaction \<lparr>interval = inte, inputs = []\<rparr> st c =
+    TransactionOutput \<lparr>txOutWarnings = newWarns, txOutPayments = newPays, txOutState = newSta, txOutContract = newCont\<rparr> \<Longrightarrow>
+    newTxOut = \<lparr>txOutWarnings = newWarns, txOutPayments = newPays, txOutState = newSta, txOutContract = newCont\<rparr> \<Longrightarrow> False"
+  (*
+  by (metis computeEmptyTransactionWarningIsCounterExample const.cases noCounterExamplePropagatesComputeEmptyTransaction)
+  *)
+  oops
+
+lemma staticAnalysisComplete_singleInputTransaction : "(\<And>c st p.
+        (\<And>t2 x. \<not> isCounterExample (execute (wrapper c t2 (Some st)) x)) \<Longrightarrow>
+        hasWarnings (playTraceAux \<lparr>txOutWarnings = [], txOutPayments = p, txOutState = st, txOutContract = c\<rparr> t) \<Longrightarrow> False) \<Longrightarrow>
+    traceListToSingleInput t2 = \<lparr>interval = inte, inputs = [inp]\<rparr> # t \<Longrightarrow>
+    (\<And>t2 x. \<not> isCounterExample (execute (wrapper c t2 (Some st)) x)) \<Longrightarrow>
+    hasWarnings (playTraceAux \<lparr>txOutWarnings = newWarns, txOutPayments = p @ newPays, txOutState = newSta, txOutContract = newCont\<rparr> t) \<Longrightarrow>
+    computeTransaction \<lparr>interval = inte, inputs = [inp]\<rparr> st c =
+    TransactionOutput \<lparr>txOutWarnings = newWarns, txOutPayments = newPays, txOutState = newSta, txOutContract = newCont\<rparr> \<Longrightarrow>
+    newTxOut = \<lparr>txOutWarnings = newWarns, txOutPayments = newPays, txOutState = newSta, txOutContract = newCont\<rparr> \<Longrightarrow> False"
+  (*
+  apply (cases newWarns)
+  apply (simp only:refl)
+  apply (metis noCounterExamplePropagatesComputeSingleInputTransaction small_lazy'.cases)
+  apply (simp only:refl)
+  by (metis computeSingleInputTransactionWarningIsCounterExample list.distinct(1) prod.exhaust)
+  *)
+  oops
+
+lemma staticAnalysisComplete_aux : "(\<And> t2 x. \<not> ( isCounterExample (execute (wrapper c t2 (Some st)) x))) \<Longrightarrow> hasWarnings (playTraceAux \<lparr>txOutWarnings = [], txOutPayments = p, txOutState = st, txOutContract = c\<rparr> t) \<Longrightarrow> False"
+  (*
+  apply (simp only:playTraceAuxToSingleInputIsEquivalent[of _ t])
+  apply (induction "traceListToSingleInput t" arbitrary: c st p t)
+  apply simp
+  subgoal for h t t2 c st p
+    apply (cases h)
+    subgoal for inte inp
+      apply (cases inp)
+      apply (subst (asm) eq_commute[of "h # t" "traceListToSingleInput t2"])
+      apply (simp only:playTraceAux.simps refl)
+      apply (cases "computeTransaction h st c")
+      subgoal for newTxOut
+        apply (cases "newTxOut")
+        subgoal for newWarns newPays newSta newCont
+          apply (simp del:computeTransaction.simps execute.simps wrapper.simps)
+          by (metis staticAnalysisComplete_emptyTransaction transactionPrefixForSingleInput)
+        done
+      apply simp
+      subgoal for inp_h inp_t
+        apply (cases "inp_t = []")
+        apply (subst (asm) eq_commute[of "h # t" "traceListToSingleInput t2"])
+        apply (simp only:playTraceAux.simps refl)
+        apply (cases "computeTransaction h st c")
+        subgoal for newTxOut
+          apply (cases "newTxOut")
+          subgoal for newWarns newPays newSta newCont
+            apply (simp del:computeTransaction.simps execute.simps wrapper.simps)
+            by (metis staticAnalysisComplete_singleInputTransaction transactionPrefixForSingleInput)
+          done
+          apply simp
+        apply (simp only:refl)
+        using traceListToSingleInput_isSingleInput by blast
+      done
+    done
+  done
+  *)
+  oops
+
+theorem staticAnalysisComplete : "(\<exists> t. hasWarnings (playTraceAux \<lparr> txOutWarnings = Nil
+                                                                  , txOutPayments = Nil
+                                                                  , txOutState = st
+                                                                  , txOutContract = c \<rparr> t)) \<Longrightarrow>
+                                  (\<exists> t x. isCounterExample (execute (wrapper c t (Some st)) x))"
+  (* using staticAnalysisComplete_aux by blast *)
+  oops
+
+theorem staticAnalysisSound : "(\<exists> t x. isCounterExample (execute (wrapper c t (Some st)) x)) \<Longrightarrow>
                                (\<exists> t. hasWarnings (playTraceAux \<lparr> txOutWarnings = Nil
                                                                , txOutPayments = Nil
                                                                , txOutState = st
                                                                , txOutContract = c \<rparr> t))"
   oops
 
+theorem staticAnalysisWorks : "(\<exists> t x. isCounterExample (execute (wrapper c t (Some st)) x)) =
+                               (\<exists> t. hasWarnings (playTraceAux \<lparr> txOutWarnings = Nil
+                                                               , txOutPayments = Nil
+                                                               , txOutState = st
+                                                               , txOutContract = c \<rparr> t))"
+  (* using staticAnalysisComplete staticAnalysisSound by blast *)
+  oops
 
 end
